ironing out some trivial errors and typos, beginning of verification effort with new ODH indexing

secure_api/box/Box.fst
@@ -88,90 +88,52 @@ assume val box_key_log:  MM.t box_key_log_region box_key_log_key box_key_log_ran
 (**
    A PKAE public key, containing a DH public key.
 *)
-noeq type pkae_pkey (pk_id:id{DH_id? pk_id}) =
-  | PKey: dh_pk:dh_pkey{ODH.pk_get_index dh_pk=pk_id} -> pkae_pkey pk_id
+type pkae_pkey = dh_pkey
 
 (**
    A PKAE private key, containing a DH private key.
 *)
-noeq abstract type pkae_skey (sk_id:id{DH_id? sk_id}) =
-  | SKey: dh_sk:dh_skey{ODH.sk_get_index dh_sk=sk_id} -> pkae_pk:pkae_pkey sk_id -> pkae_skey sk_id
+abstract type pkae_skey = dh_skey
 
 (**
    Generate a PKAE keypair, consisting of a public and a private key.
 *)
-val keygen: #(i:id{DH_id? i}) -> ST (pkae_pkey i * pkae_skey i)
-  (requires (fun h0 -> 
-    fresh i h0
-    /\ registered i
-  ))
-  (ensures (fun h0 res h1 -> 
-    unfresh i
-    /\ modifies (Set.singleton id_log_region) h0 h1
-  ))
-let keygen #i =
-  let (dh_pk, dh_sk) = ODH.keygen #i in
-  let pkae_pk = PKey #i dh_pk in
-  pkae_pk, SKey #i dh_sk pkae_pk
+let keygen = ODH.keygen
 
 (**
    Log invariant: WIP
 *)
 
-// TODO: We should be able to replace "dishonest i"  with "~(honest i)" everywhere!
-// TODO: Add patterns to quantifiers.
 let log_invariant_all_keys (h:mem) = 
-  // Removed this and made it a requirement only for the id that is currently handled.
-  //(forall (i:id{AE_id? i /\ honest i}) . MM.defined box_key_log i h <==> MM.defined dh_key_log i h) // dh_key_log and box_key_log are in sync
-  // Removed this and made it a requirement only for the id that is currently handled.
-  ///\ (forall (i:id{AE_id? i /\ honest i}) . MM.fresh box_key_log i h <==> fresh i h) // all honest keys must be present in the box_key_log
   (forall (i:id{AE_id? i /\ honest i /\ MM.defined box_key_log i h}) . let k = MM.value box_key_log i h in // if it is in the box_key_log, then the local key_log
   								let k_log = get_logGT k in          // should be contained in the heap.
 								MR.m_contains k_log h)
   /\ (forall (i:id{AE_id? i /\ honest i /\ MM.defined box_key_log i h}) (n:nonce) . let k = MM.value box_key_log i h in // if it is in the box_key_log, then box_log and the local key_log
   									    let k_log = get_logGT k in          // should be in sync.
   									    MM.defined box_log (n,i) h <==> MM.defined k_log n h)
-  // Removed this and made it a requirement only for the id that is currently handled.
-  ///\ (forall (i:id{AE_id? i /\ honest i}) (n:nonce) . (MM.fresh box_key_log i h ==> MM.fresh box_log (n,i) h)) // if it is not in the box_key_log, then there should be no nonces recorded in the box_log
 
 let log_invariant_id (h:mem) (i:id) =
   MR.m_sel h box_key_log == MR.m_sel h dh_key_log
   /\ ((AE_id? i /\ honest i) ==> (MM.fresh dh_key_log i h <==> fresh i h)) // dh_key_log and box_key_log are in sync
-  /\ (AE_id? i /\ honest i /\ MM.fresh box_key_log i h) ==> (forall (n:nonce) . (MM.fresh box_log (n,i) h)) // if it is not in the box_key_log, then there should be no nonces recorded in the box_log
+  /\ ((AE_id? i /\ honest i /\ MM.fresh box_key_log i h) ==> (forall (n:nonce) . (MM.fresh box_log (n,i) h))) // if it is not in the box_key_log, then there should be no nonces recorded in the box_log
 
 let log_invariant_single_key (h:mem) (i:id) (k:AE.key) =
   ((AE_id? i /\ honest i /\  MM.defined box_key_log i h) ==> (let k_log = get_logGT k in MR.m_contains k_log h))
-  /\ ((AE_id? i /\ honest i /\ MM.defined box_key_log i h) ==> (forall (n:nonce) . let k_log = get_logGT k in
-  										      MM.defined box_log (n,i) h <==> MM.defined k_log n h))
-
-private val recall_global_logs: unit -> ST unit
-  (requires (fun h0 -> True))
-  (ensures (fun h0 _ h1 -> 
-    h0 == h1
-    /\ MR.m_contains id_log h1
-    /\ MR.m_contains box_log h1
-    /\ MR.m_contains box_key_log h1
-    /\ MR.m_contains dh_key_log h1
-  ))
-let recall_global_logs () =
-  MR.m_recall id_log;
-  MR.m_recall dh_key_log;
-  MR.m_recall box_log;
-  MR.m_recall box_key_log
+  /\ ((AE_id? i /\ honest i /\ MM.defined box_key_log i h) ==> (forall (n:nonce) . let k_log = get_logGT k in MM.defined box_log (n,i) h ==> MM.defined k_log n h))
 
 
+#reset-options
+#set-options "--z3rlimit 200 --max_ifuel 8 --max_fuel 8"
 (**
    box_beforenm is used to generate a key using a DH public and private key. The AE id of the resulting key is a combination of the DH ids of the
    DH keys used to generate it. If idealized, the key resulting from this function will be random if both DH key ids are honest. To ensure that
    only one key is generated per DH id pair, it is stored in the box_key_log and a lookup is performed before each key is generated.
 *)
-val box_beforenm: #(pk_id:id{DH_id? pk_id /\ registered pk_id}) -> 
-	              #(sk_id:id{DH_id? sk_id /\ registered sk_id}) -> 
-	              pk:pkae_pkey pk_id -> 
-	              sk:pkae_skey sk_id ->
-		      ST (k:AE.key)
+val box_beforenm: pk:pkae_pkey -> 
+	          sk:pkae_skey ->
+		  ST (k:AE.key)
   (requires (fun h0 -> 
-    let i = generate_ae_id pk_id sk_id in
+    let i = generate_ae_id (DH_id (pk_get_share pk)) (DH_id (sk_get_share sk)) in
     registered i
     // Sync of box_log and all local key_logs
     /\ log_invariant_all_keys h0
@@ -190,13 +152,13 @@ val box_beforenm: #(pk_id:id{DH_id? pk_id /\ registered pk_id}) ->
     /\ ((AE_id? i /\ honest i /\ MM.fresh box_key_log i h0) ==> (forall (n:nonce) . (MM.fresh box_log (n,i) h0))) // if it is not in the box_key_log, then there should be no nonces recorded in the box_log
   ))
   (ensures (fun h0 k h1 -> 
-    let i = generate_ae_id pk_id sk_id in
+    let i = generate_ae_id (DH_id (pk_get_share pk)) (DH_id (sk_get_share sk)) in
     let regions_modified_dishonest = [id_log_region] in
     let regions_modified_honest_set = Set.as_set (regions_modified_dishonest @ [dh_key_log_region;box_key_log_region]) in
     let regions_modified_dishonest_set:Set.set (r:HH.rid) = Set.as_set regions_modified_dishonest in
     let k_log = get_logGT k in
     // Id sanity
-    (AE.get_index k = generate_ae_id pk_id sk_id)
+    (AE.get_index k = generate_ae_id (DH_id (pk_get_share pk)) (DH_id (sk_get_share sk)))
     // If honest, something is inserted into the log
     /\ ((AE_id?i /\ honest i) (*x*)
       ==> (let current_log = MR.m_sel h0 box_key_log in
@@ -212,15 +174,12 @@ val box_beforenm: #(pk_id:id{DH_id? pk_id /\ registered pk_id}) ->
     // If dishonest, the returned key is actually computed from both DH keys.
     /\ (dishonest i (*x*)
       ==> (modifies regions_modified_dishonest_set h0 h1
-         /\ leak_key k = ODH.prf_odhGT sk.dh_sk pk.dh_pk))
+         /\ leak_key k = ODH.prf_odhGT sk pk))
     //// Sync of box_log and the local log of the returned key
-    // TODO: This does not work yet, although it does when it's the only postcondition.
     /\ log_invariant_single_key h1 i k
     //// id is fresh if it is in the box_key_log, 
     //// sync between box_key_log and dh_key_log and
     //// if id is fresh, then there are no entries for it in the box_log
-    //// TODO: This makes only sense if we demand it for all ids. For performance reasons, 
-    //// this is currently only for the id used in this function
     /\ log_invariant_id h1 i (*x*)
     //// Liveness of global logs and local key log of the returned key.
     /\ MR.m_contains k_log h1 (*x*)
@@ -232,33 +191,21 @@ val box_beforenm: #(pk_id:id{DH_id? pk_id /\ registered pk_id}) ->
     // Would like to ensure for all keys, but verification takes too much time. Need a smarter invariant (via patterns?).
     ///\ log_invariant_all_keys h1
   ))
-let box_beforenm #pk_id #sk_id pk sk =
+let box_beforenm pk sk =
   MR.m_recall id_log;
   MR.m_recall id_honesty_log;
   MR.m_recall dh_key_log;
   MR.m_recall box_log;
   MR.m_recall box_key_log;
-  let i = generate_ae_id pk_id sk_id in
-  let h0 = ST.get() in
-  let k = prf_odh sk.dh_sk pk.dh_pk in
-  MR.m_recall id_log;
-  MR.m_recall id_honesty_log;
-  MR.m_recall dh_key_log;
-  MR.m_recall box_log;
-  MR.m_recall box_key_log;
+  let i = generate_ae_id (DH_id (pk_get_share pk)) (DH_id (sk_get_share sk)) in
+  let k = prf_odh sk pk in
   recall_log k;
   (if is_honest i then
     match MM.lookup box_key_log i with
     | Some _ ->
-      let h1 = ST.get() in
-      assert((AE_id? i /\ honest i) ==> MM.contains dh_key_log i k h1);
-      assert((AE_id? i /\ honest i) ==> MM.contains box_key_log i k h1);
       ()
     | None -> 
       MM.extend box_key_log i k;
-      let h1 = ST.get() in
-      assert(honest i ==> MM.contains dh_key_log i k h1);
-      assert(honest i ==> MM.contains box_key_log i k h1);
       ());
   recall_log k;
   MR.m_recall id_log;
@@ -266,19 +213,9 @@ let box_beforenm #pk_id #sk_id pk sk =
   MR.m_recall dh_key_log;
   MR.m_recall box_log;
   MR.m_recall box_key_log;
-  let h1 = ST.get() in
-  //assert(  let regions_modified_dishonest = [id_log_region] in
-  //  let regions_modified_honest_set = Set.as_set (regions_modified_dishonest @ [dh_key_log_region;box_key_log_region]) in
-  //  let regions_modified_dishonest_set:Set.set (r:HH.rid) = Set.as_set regions_modified_dishonest in
-  //  dishonest i ==> (modifies regions_modified_dishonest_set h0 h1 /\ makes_unfresh_just i h0 h1 /\ AE.leak_key k = prf_odhGT sk.dh_sk pk.dh_pk ));
-  //let h = ST.get() in
-  //assert(log_invariant_single_key h i k);
-  //admit();
   k
 
 
-#reset-options
-#set-options "--z3rlimit 200 --max_ifuel 8 --max_fuel 8"
 (**
    box_afternm is used to encrypt a plaintext under an AE key using a nonce. If idealized and if the AE id is honest,
    the plaintext is stored in the box_log indexed by the AE id and the nonce.
@@ -321,24 +258,24 @@ val box_afternm: k:AE.key ->
     ((dishonest i \/ ~(b2t pkae))
       ==> (c = SPEC.secretbox_easy (PlainBox.repr p) (AE.get_keyGT k) n))
     // If honest and idealizing, we encrypt zeros.
-    ///\ ((honest i /\ b2t pkae)
-    //  ==> (c == SPEC.secretbox_easy (AE.create_zero_bytes (length p)) (AE.get_keyGT k) n))
-    //// We have put the message both in the local key log and in the box_log
-    ///\ MR.witnessed (MM.contains k_log n (c,AE.message_wrap p))
-    /////\ MR.witnessed (MM.contains box_log (n,i) (c,p))
-    //// Liveness of global logs and the local key log.
-    ///\ MR.m_contains id_log h1
-    ///\ MR.m_contains id_honesty_log h1
-    ///\ MR.m_contains box_log h1
-    ///\ MR.m_contains box_key_log h1
-    ///\ MR.m_contains dh_key_log h1
-    ///\ MR.m_contains k_log h1
-    //// id is fresh if it is in the box_key_log, 
-    //// sync between box_key_log and dh_key_log and
-    //// if id is fresh, then there are no entries for it in the box_log
-    ///\ log_invariant_single_key h1 i k
-    //// Sync of box_log and the local log of the returned key
-    ///\ log_invariant_id h1 i
+    /\ ((honest i /\ b2t pkae)
+      ==> (c == SPEC.secretbox_easy (AE.create_zero_bytes (length p)) (AE.get_keyGT k) n))
+    // We have put the message both in the local key log and in the box_log
+    /\ MR.witnessed (MM.contains k_log n (c,AE.message_wrap p))
+    ///\ MR.witnessed (MM.contains box_log (n,i) (c,p))
+    // Liveness of global logs and the local key log.
+    /\ MR.m_contains id_log h1
+    /\ MR.m_contains id_honesty_log h1
+    /\ MR.m_contains box_log h1
+    /\ MR.m_contains box_key_log h1
+    /\ MR.m_contains dh_key_log h1
+    /\ MR.m_contains k_log h1
+    // id is fresh if it is in the box_key_log, 
+    // sync between box_key_log and dh_key_log and
+    // if id is fresh, then there are no entries for it in the box_log
+    /\ log_invariant_single_key h1 i k
+    // Sync of box_log and the local log of the returned key
+    /\ log_invariant_id h1 i
   ))
 let box_afternm k n p =
   MR.m_recall id_honesty_log;
@@ -351,11 +288,6 @@ let box_afternm k n p =
   fresh_unfresh_contradiction i;
   let ae_m = AE.message_wrap #i p in
   let c = AE.encrypt #i n k ae_m in
-  MR.m_recall id_honesty_log;
-  MR.m_recall box_key_log;
-  MR.m_recall id_log;
-  MR.m_recall dh_key_log;
-  MR.m_recall box_log;
   let honest_i = is_honest i in
   (if honest_i then
     MM.extend box_log (n,i) (c,p));
@@ -373,10 +305,10 @@ val box: #(pk_id:id{DH_id? pk_id}) ->
 	     pk:pkae_pkey pk_id{registered pk_id} -> 
 	     sk:pkae_skey sk_id{registered sk_id} -> 
 	     n:nonce -> 
-	     p:protected_pkae_plain{PlainPKAE.get_index p = generate_ae_id pk_id sk_id} 
+	     p:protected_pkae_plain{PlainPKAE.get_index p = generate_ae_id (DH_id (pk_get_share pk)) (DH_id (sk_get_share sk))} 
 	     -> ST c
   (requires (fun h0 ->
-    let i = generate_ae_id pk_id sk_id in
+    let i = generate_ae_id (DH_id (pk_get_share pk)) (DH_id (sk_get_share sk)) in
     registered i
     // Liveness of global logs
     /\ MR.m_contains id_log h0
@@ -391,11 +323,10 @@ val box: #(pk_id:id{DH_id? pk_id}) ->
     /\ MM.fresh box_log (n,i) h0
   ))
   (ensures (fun h0 c h1 -> 
-    let i = generate_ae_id pk_id sk_id in
+    let i = generate_ae_id (DH_id (pk_get_share pk)) (DH_id (sk_get_share sk)) in
     // Make sure that log_invariants hold. Would like to ensure "all_keys" variant, but too expensive to verify currently.
     log_invariant_id h1 i
-    // TODO: Proof via reasoning over h1
-    ///\ log_invariant_single_key h1 i k
+    /\ log_invariant_single_key h1 i k
     /\ MR.m_contains id_log h1
     /\ MR.m_contains id_honesty_log h1
     /\ MR.m_contains box_log h1
@@ -416,7 +347,7 @@ val box_open: #(sk_id:id{DH_id? sk_id}) ->
 	     c:cipher ->
 	     ST(option (p:protected_pkae_plain))
   (requires (fun h0 ->
-    let i = generate_ae_id pk_id sk_id in
+    let i = generate_ae_id (DH_id (pk_get_share pk)) (DH_id (sk_get_share sk)) in
     registered i
     // Liveness of global logs
     /\ MR.m_contains box_log h0
@@ -429,7 +360,7 @@ val box_open: #(sk_id:id{DH_id? sk_id}) ->
     /\ log_invariant_id h0 i
   ))
   (ensures (fun h0 p h1 -> 
-    let i = generate_ae_id pk_id sk_id in
+    let i = generate_ae_id (DH_id (pk_get_share pk)) (DH_id (sk_get_share sk)) in
     // Make sure that log_invariants hold. Would like to ensure "all_keys" variant, but too expensive to verify currently.
     log_invariant_id h1 i
     /\ log_invariant_all_keys h1
@@ -437,7 +368,6 @@ val box_open: #(sk_id:id{DH_id? sk_id}) ->
 let box_open #sk_id #pk_id n sk pk c =
   let k = box_beforenm #pk_id #sk_id pk sk in
   let i = AE.get_index k in
-  // TODO : perform lookup in box_log
   match AE.decrypt #i n k c with
   | Some p -> 
     let p' = (AE.message_unwrap #i p) in 
